`StateGettersEquivalence`: add proofs for `GASLIMIT` and `CHAINID`

EvmEquivalence/Equivalence/StateGettersEquivalence.lean
@@ -21,6 +21,8 @@ inductive stateGetter_op where
   | timestamp
   | number
   | prevrandao
+  | gaslimit
+  | chainid
 
 variable (op : stateGetter_op)
 
@@ -34,6 +36,8 @@ def stateGetter_op.to_binop : stateGetter_op → SortNullStackOp
   | .timestamp => .TIMESTAMP_EVM_NullStackOp
   | .number => .NUMBER_EVM_NullStackOp
   | .prevrandao => .PREVRANDAO_EVM_NullStackOp
+  | .gaslimit => .GASLIMIT_EVM_NullStackOp
+  | .chainid => .CHAINID_EVM_NullStackOp
 
 def stateGetter_op.from_k : stateGetter_op → StateGettersSummary.stateGetter_op
  | .address  => .address
@@ -44,11 +48,13 @@ def stateGetter_op.from_k : stateGetter_op → StateGettersSummary.stateGetter_o
  | .timestamp => .timestamp
  | .number => .number
  | .prevrandao => .prevrandao
+ | .gaslimit => .gaslimit
+ | .chainid => .chainid
 
 def oneOpLHS
-  {GAS_CELL ID_CELL ORIGIN_CELL CALLER_CELL COINBASE_CELL TIMESTAMP_CELL MIXHASH_CELL NUMBER_CELL PC_CELL _Val6 _Val8 : SortInt}
+  {GAS_CELL ID_CELL ORIGIN_CELL CALLER_CELL GASPRICE_CELL  COINBASE_CELL TIMESTAMP_CELL MIXHASH_CELL NUMBER_CELL GASLIMIT_CELL CHAINID_CELL PC_CELL _Val6 _Val8 : SortInt}
   -- We assume `GASPRICE_CELL` is not negative
-  {GASPRICE_CELL : ℕ}
+  --{GASPRICE_CELL : ℕ}
   {SCHEDULE_CELL : SortSchedule}
   {USEGAS_CELL: SortBool}
   {WS : SortWordStack}
@@ -112,15 +118,18 @@ def oneOpLHS
                     coinbase := { val := COINBASE_CELL},
                     timestamp := { val := TIMESTAMP_CELL },
                     number := { val := NUMBER_CELL },
+                    gasLimit := { val := GASLIMIT_CELL },
                     mixHash := { val := MIXHASH_CELL }
                     } },
-        network := _DotVar2 } },
+        network := {_DotVar2 with
+                      chainID := { val := CHAINID_CELL }
+                      } } },
     generatedCounter := _DotVar0 }
 
 def oneOpRHS
-  {TOP_STACK ID_CELL ORIGIN_CELL CALLER_CELL COINBASE_CELL TIMESTAMP_CELL MIXHASH_CELL NUMBER_CELL _Val6 _Val8 : SortInt}
+  {TOP_STACK ID_CELL ORIGIN_CELL CALLER_CELL GASPRICE_CELL  COINBASE_CELL TIMESTAMP_CELL MIXHASH_CELL NUMBER_CELL GASLIMIT_CELL CHAINID_CELL _Val6 _Val8 : SortInt}
   -- We assume `GASPRICE_CELL` is not negative
-  {GASPRICE_CELL : ℕ}
+  --{GASPRICE_CELL : ℕ}
   {SCHEDULE_CELL : SortSchedule}
   {WS : SortWordStack}
   {_DotVar0 : SortGeneratedCounterCell}
@@ -183,9 +192,12 @@ def oneOpRHS
                     coinbase := { val := COINBASE_CELL},
                     timestamp := { val := TIMESTAMP_CELL },
                     number := { val := NUMBER_CELL },
+                    gasLimit := { val := GASLIMIT_CELL },
                     mixHash := { val := MIXHASH_CELL },
                     } },
-          network := _DotVar2 } },
+          network := {_DotVar2 with
+                      chainID := { val := CHAINID_CELL }
+                      } } },
       generatedCounter := _DotVar0 }
 
 @[simp]
@@ -208,11 +220,13 @@ def stateGetter_op.do (tc : SortGeneratedTopCell) : SortInt :=
   | .timestamp => tc.timestamp.val
   | .number => tc.number.val
   | .prevrandao => tc.mixhash.val
+  | .gaslimit => tc.gaslimit.val
+  | .chainid => tc.chainid.val -- This doesn't exist in EvmYul state
 
 theorem rw_oneOpLHS_oneOpRHS
-  {GAS_CELL ID_CELL ORIGIN_CELL CALLER_CELL COINBASE_CELL TIMESTAMP_CELL MIXHASH_CELL NUMBER_CELL PC_CELL _Val0 _Val2 _Val6 _Val7 _Val8 : SortInt}
+  {GAS_CELL ID_CELL ORIGIN_CELL CALLER_CELL GASPRICE_CELL  COINBASE_CELL TIMESTAMP_CELL MIXHASH_CELL NUMBER_CELL GASLIMIT_CELL CHAINID_CELL PC_CELL _Val0 _Val2 _Val6 _Val7 _Val8 : SortInt}
   -- We assume `GASPRICE_CELL` is not negative
-  {GASPRICE_CELL : ℕ}
+  --{GASPRICE_CELL : ℕ}
   {SCHEDULE_CELL : SortSchedule}
   {USEGAS_CELL _Val1 _Val3 _Val4 _Val5 : SortBool}
   {WS : SortWordStack}
@@ -250,13 +264,13 @@ theorem rw_oneOpLHS_oneOpRHS
   (defn_Val7 : «_<_>_SCHEDULE_Int_ScheduleConst_Schedule» SortScheduleConst.Gbase_SCHEDULE_ScheduleConst SCHEDULE_CELL = some _Val7)
   (defn_Val8 : «_-Int_» GAS_CELL _Val7 = some _Val8)
   (req : _Val5 = true):
-  let lhs := (@oneOpLHS op GAS_CELL ID_CELL ORIGIN_CELL CALLER_CELL COINBASE_CELL TIMESTAMP_CELL MIXHASH_CELL NUMBER_CELL PC_CELL _Val6 _Val8 GASPRICE_CELL SCHEDULE_CELL USEGAS_CELL WS _DotVar0 _DotVar2 _Gen0 _Gen1 _Gen10
+  let lhs := (@oneOpLHS op GAS_CELL ID_CELL ORIGIN_CELL CALLER_CELL GASPRICE_CELL  COINBASE_CELL TIMESTAMP_CELL MIXHASH_CELL NUMBER_CELL GASLIMIT_CELL CHAINID_CELL PC_CELL _Val6 _Val8 /- GASPRICE_CELL -/  SCHEDULE_CELL USEGAS_CELL WS _DotVar0 _DotVar2 _Gen0 _Gen1 _Gen10
   _Gen11 _Gen12 _Gen13 _Gen14 _Gen15 _Gen16 _Gen19
   _Gen20 _Gen21 _Gen22 _Gen3 _Gen4 _Gen5 _Gen6 _Gen7 _Gen8 _Gen9 _K_CELL)
-  let rhs := (@oneOpRHS (op.do lhs) ID_CELL ORIGIN_CELL CALLER_CELL COINBASE_CELL TIMESTAMP_CELL MIXHASH_CELL NUMBER_CELL _Val6 _Val8 GASPRICE_CELL SCHEDULE_CELL WS _DotVar0 _DotVar2 _Gen0 _Gen1 _Gen10 _Gen11 _Gen12 _Gen13 _Gen14 _Gen15 _Gen16 _Gen19 _Gen20 _Gen21 _Gen22 _Gen3 _Gen4 _Gen5 _Gen6 _Gen7 _Gen8 _Gen9 _K_CELL)
+  let rhs := (@oneOpRHS (op.do lhs) ID_CELL ORIGIN_CELL CALLER_CELL GASPRICE_CELL  COINBASE_CELL TIMESTAMP_CELL MIXHASH_CELL NUMBER_CELL GASLIMIT_CELL CHAINID_CELL _Val6 _Val8 /- GASPRICE_CELL -/ SCHEDULE_CELL WS _DotVar0 _DotVar2 _Gen0 _Gen1 _Gen10 _Gen11 _Gen12 _Gen13 _Gen14 _Gen15 _Gen16 _Gen19 _Gen20 _Gen21 _Gen22 _Gen3 _Gen4 _Gen5 _Gen6 _Gen7 _Gen8 _Gen9 _K_CELL)
   Rewrites lhs rhs
    := by
-  --intro lhs rhs; simp [lhs, rhs, oneOpLHS, oneOpRHS]
+  intro lhs rhs; simp [lhs, rhs, oneOpLHS, oneOpRHS]
   cases op
   . apply (@Rewrites.ADDRESS_SUMMARY_ADDRESS_SUMMARY_USEGAS GAS_CELL ID_CELL PC_CELL _Val0 _Val2)
     <;> assumption
@@ -274,11 +288,15 @@ theorem rw_oneOpLHS_oneOpRHS
     <;> try assumption
   . apply (@Rewrites.PREVRANDAO_SUMMARY_PREVRANDAO_SUMMARY_USEGAS GAS_CELL MIXHASH_CELL PC_CELL _Val0 _Val2)
     <;> try assumption
+  . apply (@Rewrites.GASLIMIT_SUMMARY_GASLIMIT_SUMMARY_USEGAS GASLIMIT_CELL GAS_CELL PC_CELL _Val0 _Val2)
+    <;> try assumption
+  . apply (@Rewrites.CHAINID_SUMMARY_CHAINID_SUMMARY_USEGAS CHAINID_CELL GAS_CELL PC_CELL _Val0 _Val2)
+    <;> try assumption
 
 theorem oneOp_prestate_equiv
-  {GAS_CELL ID_CELL ORIGIN_CELL CALLER_CELL COINBASE_CELL TIMESTAMP_CELL MIXHASH_CELL NUMBER_CELL PC_CELL _Val6 _Val8 : SortInt}
+  {GAS_CELL ID_CELL ORIGIN_CELL CALLER_CELL GASPRICE_CELL  COINBASE_CELL TIMESTAMP_CELL MIXHASH_CELL NUMBER_CELL GASLIMIT_CELL CHAINID_CELL PC_CELL _Val6 _Val8 : SortInt}
   -- We assume `GASPRICE_CELL` is not negative
-  {GASPRICE_CELL : ℕ}
+  --{GASPRICE_CELL : ℕ}
   {SCHEDULE_CELL : SortSchedule}
   {USEGAS_CELL: SortBool}
   {WS : SortWordStack}
@@ -306,7 +324,7 @@ theorem oneOp_prestate_equiv
   {_Gen9 : SortCallDepthCell}
   {_K_CELL : SortK}
   (symState : EVM.State):
-  let lhs := (@oneOpLHS op GAS_CELL ID_CELL ORIGIN_CELL CALLER_CELL COINBASE_CELL TIMESTAMP_CELL MIXHASH_CELL NUMBER_CELL PC_CELL _Val6 _Val8 GASPRICE_CELL SCHEDULE_CELL USEGAS_CELL WS _DotVar0 _DotVar2 _Gen0 _Gen1 _Gen10
+  let lhs := (@oneOpLHS op GAS_CELL ID_CELL ORIGIN_CELL CALLER_CELL GASPRICE_CELL  COINBASE_CELL TIMESTAMP_CELL MIXHASH_CELL NUMBER_CELL GASLIMIT_CELL CHAINID_CELL PC_CELL _Val6 _Val8 /- GASPRICE_CELL -/ SCHEDULE_CELL USEGAS_CELL WS _DotVar0 _DotVar2 _Gen0 _Gen1 _Gen10
   _Gen11 _Gen12 _Gen13 _Gen14 _Gen15 _Gen16 _Gen19
   _Gen20 _Gen21 _Gen22 _Gen3 _Gen4 _Gen5 _Gen6 _Gen7 _Gen8 _Gen9 _K_CELL)
   stateMap symState lhs =
@@ -315,13 +333,6 @@ theorem oneOp_prestate_equiv
     pc := intMap PC_CELL
     gasAvailable := intMap GAS_CELL
     executionEnv := executionEnv_map lhs symState
-    /- {symState.executionEnv with
-                  code := _Gen0.val,
-                  codeOwner := idMap lhs.Iₐ
-                  sender := accountAddressMap lhs.origin.val
-                  source := accountAddressMap lhs.caller.val
-                  gasPrice := GASPRICE_CELL
-                  perm := !lhs.isStatic.val} -/
     accountMap := Axioms.SortAccountsCellMap lhs.accounts
     activeWords := intMap lhs.memoryUsed.val
     memory := memory_map lhs.memory
@@ -335,9 +346,9 @@ theorem oneOp_prestate_equiv
     simp [oneOpLHS, cop, stateMap, stateGetter_op.from_k] <;> rfl
 
 theorem oneOp_poststate_equiv
-  {TOP_STACK ID_CELL ORIGIN_CELL CALLER_CELL COINBASE_CELL TIMESTAMP_CELL MIXHASH_CELL NUMBER_CELL PC_CELL _Val5 _Val6 _Val8 : SortInt}
+  {TOP_STACK ID_CELL ORIGIN_CELL CALLER_CELL GASPRICE_CELL  COINBASE_CELL TIMESTAMP_CELL MIXHASH_CELL NUMBER_CELL GASLIMIT_CELL CHAINID_CELL PC_CELL _Val5 _Val6 _Val8 : SortInt}
   -- We assume `GASPRICE_CELL` is not negative
-  {GASPRICE_CELL : ℕ}
+  --{GASPRICE_CELL : ℕ}
   {SCHEDULE_CELL : SortSchedule}
   {WS : SortWordStack}
   {_DotVar0 : SortGeneratedCounterCell}
@@ -365,20 +376,13 @@ theorem oneOp_poststate_equiv
   {_K_CELL : SortK}
   (defn_Val6 : «_+Int_» PC_CELL 1 = some _Val6)
   (symState : EVM.State):
-  let rhs := (@oneOpRHS TOP_STACK ID_CELL ORIGIN_CELL CALLER_CELL COINBASE_CELL TIMESTAMP_CELL MIXHASH_CELL NUMBER_CELL _Val6 _Val8 GASPRICE_CELL SCHEDULE_CELL WS _DotVar0 _DotVar2 _Gen0 _Gen1 _Gen10 _Gen11 _Gen12 _Gen13 _Gen14 _Gen15 _Gen16 _Gen19 _Gen20 _Gen21 _Gen22 _Gen3 _Gen4 _Gen5 _Gen6 _Gen7 _Gen8 _Gen9 _K_CELL)
+  let rhs := (@oneOpRHS TOP_STACK ID_CELL ORIGIN_CELL CALLER_CELL GASPRICE_CELL  COINBASE_CELL TIMESTAMP_CELL MIXHASH_CELL NUMBER_CELL GASLIMIT_CELL CHAINID_CELL _Val6 _Val8 /- GASPRICE_CELL -/ SCHEDULE_CELL WS _DotVar0 _DotVar2 _Gen0 _Gen1 _Gen10 _Gen11 _Gen12 _Gen13 _Gen14 _Gen15 _Gen16 _Gen19 _Gen20 _Gen21 _Gen22 _Gen3 _Gen4 _Gen5 _Gen6 _Gen7 _Gen8 _Gen9 _K_CELL)
   stateMap symState rhs =
   {symState with
     stack := (intMap TOP_STACK) :: wordStackMap WS
     pc := intMap (PC_CELL + 1)
     gasAvailable := intMap _Val8
     executionEnv := executionEnv_map rhs symState
-    /- {symState.executionEnv with
-                  code := _Gen0.val,
-                  codeOwner := idMap rhs.Iₐ,
-                  sender := accountAddressMap rhs.origin.val
-                  source := accountAddressMap rhs.caller.val
-                  gasPrice := GASPRICE_CELL
-                  perm := !rhs.isStatic.val} -/
     accountMap := Axioms.SortAccountsCellMap rhs.accounts
     activeWords := intMap rhs.memoryUsed.val
     memory := memory_map rhs.memory
@@ -400,9 +404,9 @@ attribute [local simp] GasConstants.Gbase
 -- We cannot prove full equivalence for the `EVM.step` function
 -- This is because it doesn't include all semantics such as gas computation
 theorem step_oneOp_equiv
-  {GAS_CELL ID_CELL ORIGIN_CELL CALLER_CELL COINBASE_CELL TIMESTAMP_CELL MIXHASH_CELL NUMBER_CELL PC_CELL _Val0 _Val2 _Val6 _Val7 _Val8 : SortInt}
+  {GAS_CELL ID_CELL ORIGIN_CELL CALLER_CELL GASPRICE_CELL  COINBASE_CELL TIMESTAMP_CELL MIXHASH_CELL NUMBER_CELL GASLIMIT_CELL PC_CELL _Val0 _Val2 _Val6 _Val7 _Val8 : SortInt}
   -- We assume `GASPRICE_CELL` is not negative
-  {GASPRICE_CELL : ℕ}
+  --{GASPRICE_CELL : ℕ}
   {SCHEDULE_CELL : SortSchedule}
   {USEGAS_CELL _Val1 _Val3 _Val4 _Val5 : SortBool}
   {WS : SortWordStack}
@@ -456,21 +460,21 @@ theorem step_oneOp_equiv
   (ORIGIN_CELL_nonneg : 0 ≤ ORIGIN_CELL)
   (CALLER_CELL_small : CALLER_CELL < AccountAddress.size)
   (CALLER_CELL_nonneg : 0 ≤ CALLER_CELL)
+  (GASPRICE_CELL_nonneg : 0 ≤ GASPRICE_CELL)
   (COINBASE_CELL_small : COINBASE_CELL < AccountAddress.size)
   (COINBASE_CELL_nonneg : 0 ≤ COINBASE_CELL)
-  (TIMESTAMP_CELL_small : TIMESTAMP_CELL < UInt256.size)
   (TIMESTAMP_CELL_nonneg : 0 ≤ TIMESTAMP_CELL)
-  (NUMBER_CELL_small : NUMBER_CELL < UInt256.size)
-  (NUMBER_CELL_nonneg : 0 ≤ NUMBER_CELL):
-  let lhs := (@oneOpLHS op GAS_CELL ID_CELL ORIGIN_CELL CALLER_CELL COINBASE_CELL TIMESTAMP_CELL MIXHASH_CELL NUMBER_CELL PC_CELL _Val6 _Val8 GASPRICE_CELL SCHEDULE_CELL USEGAS_CELL WS _DotVar0 _DotVar2 _Gen0 _Gen1 _Gen10
+  (NUMBER_CELL_nonneg : 0 ≤ NUMBER_CELL)
+  (GASLIMIT_CELL_nonneg : 0 ≤ GASLIMIT_CELL) :
+  let lhs := (@oneOpLHS op GAS_CELL ID_CELL ORIGIN_CELL CALLER_CELL GASPRICE_CELL  COINBASE_CELL TIMESTAMP_CELL MIXHASH_CELL NUMBER_CELL GASLIMIT_CELL 1 /- CHAINID_CELL -/ PC_CELL _Val6 _Val8 /- GASPRICE_CELL -/ SCHEDULE_CELL USEGAS_CELL WS _DotVar0 _DotVar2 _Gen0 _Gen1 _Gen10
   _Gen11 _Gen12 _Gen13 _Gen14 _Gen15 _Gen16 _Gen19
   _Gen20 _Gen21 _Gen22 _Gen3 _Gen4 _Gen5 _Gen6 _Gen7 _Gen8 _Gen9 _K_CELL)
-  let rhs := (@oneOpRHS (op.do lhs) ID_CELL ORIGIN_CELL CALLER_CELL COINBASE_CELL TIMESTAMP_CELL MIXHASH_CELL NUMBER_CELL _Val6 _Val8 GASPRICE_CELL  SCHEDULE_CELL WS _DotVar0 _DotVar2 _Gen0 _Gen1 _Gen10 _Gen11 _Gen12 _Gen13 _Gen14 _Gen15 _Gen16  _Gen19 _Gen20 _Gen21 _Gen22 _Gen3 _Gen4 _Gen5 _Gen6 _Gen7 _Gen8 _Gen9 _K_CELL)
+  let rhs := (@oneOpRHS (op.do lhs) ID_CELL ORIGIN_CELL CALLER_CELL GASPRICE_CELL  COINBASE_CELL TIMESTAMP_CELL MIXHASH_CELL NUMBER_CELL GASLIMIT_CELL 1 /- CHAINID_CELL -/ _Val6 _Val8 /- GASPRICE_CELL -/ SCHEDULE_CELL WS _DotVar0 _DotVar2 _Gen0 _Gen1 _Gen10 _Gen11 _Gen12 _Gen13 _Gen14 _Gen15 _Gen16  _Gen19 _Gen20 _Gen21 _Gen22 _Gen3 _Gen4 _Gen5 _Gen6 _Gen7 _Gen8 _Gen9 _K_CELL)
   EVM.step_arith op.from_k gas gasCost (stateMap symState lhs) =
   .ok (stateMap {symState with execLength := symState.execLength + 1} rhs) := by
   intro lhs rhs
   rw [oneOp_prestate_equiv]
-  rw [@oneOp_poststate_equiv _ ID_CELL ORIGIN_CELL CALLER_CELL COINBASE_CELL TIMESTAMP_CELL MIXHASH_CELL NUMBER_CELL PC_CELL]
+  rw [@oneOp_poststate_equiv _ ID_CELL ORIGIN_CELL CALLER_CELL GASPRICE_CELL  COINBASE_CELL TIMESTAMP_CELL MIXHASH_CELL NUMBER_CELL GASLIMIT_CELL 1 PC_CELL]
   <;> try assumption
   cases gas; contradiction
   case succ gas =>
@@ -483,16 +487,10 @@ theorem step_oneOp_equiv
     . rw [←UInt256.add_succ_mod_size, intMap_add_dist] <;> aesop
     . generalize h_top_stack : op.do lhs = top_stack
       cases op <;> simp [lhs, oneOpLHS, stateGetter_op.from_k] <;>
-       -- `address`
-        simp [intMap, AccountAddress.ofNat, UInt256.ofNat, Id.run, UInt256.toSigned] <;>
-        cases top_stack <;>
-        aesop (add simp [Fin.val, Fin.ofNat, AccountAddress.size, State.coinBase, State.timeStamp])
-        (add safe (by omega))
-      /- . -- `origin`
-        simp [intMap, AccountAddress.ofNat, UInt256.ofNat, Id.run, UInt256.toSigned]
-        cases top_stack <;>
-        aesop (add simp [Fin.val, Fin.ofNat, AccountAddress.size])
-        (add safe (by omega)) -/
+      simp [intMap, AccountAddress.ofNat, UInt256.ofNat, Id.run, UInt256.toSigned] <;>
+      cases top_stack <;>
+      aesop (add simp [Fin.val, Fin.ofNat, AccountAddress.size, State.coinBase, State.timeStamp])
+      (add safe (by omega))
 
 
 attribute [local simp] GasConstants.Glow
@@ -506,9 +504,9 @@ attribute [local simp] GasConstants.Glow
  6. `W0` and `W1` are nonnegative
  -/
 theorem X_oneOp_equiv
-  {GAS_CELL ID_CELL ORIGIN_CELL CALLER_CELL COINBASE_CELL TIMESTAMP_CELL MIXHASH_CELL NUMBER_CELL PC_CELL _Val0 _Val2 _Val6 _Val7 _Val8 : SortInt}
+  {GAS_CELL ID_CELL ORIGIN_CELL CALLER_CELL GASPRICE_CELL  COINBASE_CELL TIMESTAMP_CELL MIXHASH_CELL NUMBER_CELL GASLIMIT_CELL PC_CELL _Val0 _Val2 _Val6 _Val7 _Val8 : SortInt}
   -- We assume `GASPRICE_CELL` is not negative
-  {GASPRICE_CELL : ℕ}
+  --{GASPRICE_CELL : ℕ}
   {SCHEDULE_CELL : SortSchedule}
   {USEGAS_CELL _Val1 _Val3 _Val4 _Val5 : SortBool}
   {WS : SortWordStack}
@@ -560,16 +558,16 @@ theorem X_oneOp_equiv
   (ORIGIN_CELL_nonneg : 0 ≤ ORIGIN_CELL)
   (CALLER_CELL_small : CALLER_CELL < AccountAddress.size)
   (CALLER_CELL_nonneg : 0 ≤ CALLER_CELL)
+  (GASPRICE_CELL_nonneg : 0 ≤ GASPRICE_CELL)
   (COINBASE_CELL_small : COINBASE_CELL < AccountAddress.size)
   (COINBASE_CELL_nonneg : 0 ≤ COINBASE_CELL)
-  (TIMESTAMP_CELL_small : TIMESTAMP_CELL < UInt256.size)
   (TIMESTAMP_CELL_nonneg : 0 ≤ TIMESTAMP_CELL)
-  (NUMBER_CELL_small : NUMBER_CELL < UInt256.size)
-  (NUMBER_CELL_nonneg : 0 ≤ NUMBER_CELL) :
-  let lhs := (@oneOpLHS op GAS_CELL ID_CELL ORIGIN_CELL CALLER_CELL COINBASE_CELL TIMESTAMP_CELL MIXHASH_CELL NUMBER_CELL PC_CELL _Val6 _Val8 GASPRICE_CELL SCHEDULE_CELL USEGAS_CELL WS _DotVar0 _DotVar2 ⟨op.from_k.to_bin⟩ _Gen1 _Gen10
+  (NUMBER_CELL_nonneg : 0 ≤ NUMBER_CELL)
+  (GASLIMIT_CELL_nonneg : 0 ≤ GASLIMIT_CELL) :
+  let lhs := (@oneOpLHS op GAS_CELL ID_CELL ORIGIN_CELL CALLER_CELL GASPRICE_CELL  COINBASE_CELL TIMESTAMP_CELL MIXHASH_CELL NUMBER_CELL GASLIMIT_CELL 1 /- CHAINID_CELL -/ PC_CELL _Val6 _Val8 /- GASPRICE_CELL -/ SCHEDULE_CELL USEGAS_CELL WS _DotVar0 _DotVar2 ⟨op.from_k.to_bin⟩ _Gen1 _Gen10
   _Gen11 _Gen12 _Gen13 _Gen14 _Gen15 _Gen16 _Gen19
   _Gen20 _Gen21 _Gen22 _Gen3 _Gen4 _Gen5 _Gen6 _Gen7 _Gen8 _Gen9 _K_CELL)
-  let rhs := (@oneOpRHS (op.do lhs) ID_CELL ORIGIN_CELL CALLER_CELL COINBASE_CELL TIMESTAMP_CELL MIXHASH_CELL NUMBER_CELL _Val6 _Val8 GASPRICE_CELL SCHEDULE_CELL WS _DotVar0 _DotVar2 _Gen0 _Gen1 ⟨.empty⟩ _Gen11 _Gen12 _Gen13 _Gen14 _Gen15 _Gen16 _Gen19 _Gen20 _Gen21 _Gen22 _Gen3 _Gen4 _Gen5 _Gen6 _Gen7 _Gen8 _Gen9 _K_CELL)
+  let rhs := (@oneOpRHS (op.do lhs) ID_CELL ORIGIN_CELL CALLER_CELL GASPRICE_CELL  COINBASE_CELL TIMESTAMP_CELL MIXHASH_CELL NUMBER_CELL GASLIMIT_CELL 1 /- CHAINID_CELL -/ _Val6 _Val8 /- GASPRICE_CELL -/ SCHEDULE_CELL WS _DotVar0 _DotVar2 _Gen0 _Gen1 ⟨.empty⟩ _Gen11 _Gen12 _Gen13 _Gen14 _Gen15 _Gen16 _Gen19 _Gen20 _Gen21 _Gen22 _Gen3 _Gen4 _Gen5 _Gen6 _Gen7 _Gen8 _Gen9 _K_CELL)
   EVM.X (UInt256.toNat (intMap GAS_CELL)) symValidJumps
   (stateMap symState lhs) =
   .ok (.success (stateMap {symState with execLength := symState.execLength + 2} rhs) ByteArray.empty) := by
@@ -577,7 +575,7 @@ theorem X_oneOp_equiv
   -- With `simp` doesn't work
   --rw [codeDiv, pcZero]
   rw [oneOp_prestate_equiv]
-  rw [@oneOp_poststate_equiv _ ID_CELL ORIGIN_CELL CALLER_CELL COINBASE_CELL TIMESTAMP_CELL MIXHASH_CELL NUMBER_CELL PC_CELL]
+  rw [@oneOp_poststate_equiv _ ID_CELL ORIGIN_CELL CALLER_CELL GASPRICE_CELL  COINBASE_CELL TIMESTAMP_CELL MIXHASH_CELL NUMBER_CELL GASLIMIT_CELL 1 /- CHAINID_CELL -/ PC_CELL]
   <;> try assumption
   -- If we don't apply this lemma we cannot rewrite X_add_summary
   have pc_equiv : intMap 0 = UInt256.ofNat 0 := rfl
@@ -596,12 +594,10 @@ theorem X_oneOp_equiv
     (add safe (by rw [intMap_sub_dist]))
     (add safe (by apply le_of_lt))
   . generalize h_top_stack : op.do lhs = top_stack
-    cases op <;> simp [stateGetter_op.from_k]
-    --. -- `address`
-      <;>
-      cases top_stack <;> simp [oneOpLHS, intMap, AccountAddress.ofNat] <;>
-      simp [UInt256.ofNat, Id.run, UInt256.toSigned] <;>
-      aesop (add simp [Fin.val, Fin.ofNat, AccountAddress.size, State.coinBase, State.number])
-      (add safe (by omega))
+    cases op <;> simp [stateGetter_op.from_k] <;>
+    cases top_stack <;> simp [oneOpLHS, intMap, AccountAddress.ofNat] <;>
+    simp [UInt256.ofNat, Id.run, UInt256.toSigned] <;>
+    aesop (add simp [Fin.val, Fin.ofNat, AccountAddress.size, State.coinBase, State.number])
+    (add safe (by omega))
 
 end StateGettersEquivalence
